src/FlatModel.v
@@ -58,27 +58,57 @@ Definition code_writes (c : list ast) :=
                         write_footprint := {| Types.location := next_loc; Types.size := 4 |};
                         write_val := unsafe_encode a ;
                         write_kind := WKNormal |})::ws,
-                    next_wid + 1, next_loc + 4))
+                    next_wid + 1, MemLoc (mem_loc_to_nat next_loc + 4)))
                 c
-                (nil, 0, 1000) in
+                (nil, 0, MemLoc 4096) in
   ws.
 
+Definition data_writes (ds : list (nat * list nat)) :=
+  List.map (fun '(loc, bytes) =>
+              (0, 0, {| write_id := 0;
+                        write_footprint := {| Types.location := MemLoc loc;
+                                              Types.size := List.length bytes |};
+                        write_val := List.rev bytes;
+                        write_kind := WKNormal |}))
+           ds.
+
 Definition run_test (code : list (instruction_id_t * mem_write_id_t * mem_write))
-           (bound : nat) :=
-  Model.exec bound code [1000].
+           (bound : nat) : ((_ + _) * _) :=
+  Model.exec bound code [MemLoc 4096].
+
+Existing Instance Model.showable_state.
+
+Definition show_state (s : Model.state) :=
+  show s.
 
 Definition test_and :=
   code_writes [
-      (* 1000 : *) AND X0, X1, X2
-      (* 1004 : *) ; B #-1004 (* jump to 0, indicates to the model to stop fetching *)
-    ].
+      (* [0x1000] *) MOVZ X1, #1234
+      (* [0x1004] *) ; AND X0, X1, X2
+      (* [0x1008] *) ; B #-4104 (* jump to 0, indicates to the model to stop fetching *)
+    ]%a64.
+
+Definition test_str :=
+  data_writes [ (5000, [0; 0; 0; 0; 0; 0; 0; 0]) ] ++
+  code_writes [ (* [0x1000] *) MOVZ X0,#42
+                (* [0x1004] *) ; MOVZ X1,#5000
+                (* [0x1008] *) ; STR X0,[X1]
+                (* [0x100c] *) ; B #-4108 (* jump to 0, indicates to the model to stop fetching *)
+              ]%a64.
+
+Definition test_ldr :=
+  data_writes [ (5000, [0; 0; 0; 0; 0; 0; 0; 42]) ] ++
+  code_writes [ (* [0x1000] *) MOVZ X0,#5000
+                (* [0x1004] *) ; LDR X1,[X0]
+                (* [0x1008] *) ; B #-4104 (* jump to 0, indicates to the model to stop fetching *)
+              ]%a64.
 
 (* Compute match run_test test_and 5 with inr (_, s) => s | _ => [] end. *)
 
 From Coq Require
      Extraction
-     ExtrOcamlString
      ExtrOcamlBasic
+     ExtrOcamlString
      ExtrOcamlNatBigInt
      ExtrOcamlZBigInt
      ExtrOcamlIntConv.
@@ -87,7 +117,9 @@ Extraction Language OCaml.
 Extraction Blacklist Nat List.
 Cd "extracted_ocaml".
 
-Separate Extraction ExtrOcamlIntConv.nat_of_int ExtrOcamlIntConv.int_of_nat.
-Separate Extraction run_test test_and.
+Separate Extraction
+         ExtrOcamlIntConv.nat_of_int ExtrOcamlIntConv.int_of_nat
+         run_test show_state
+         test_and test_str test_ldr.
 
 Cd "..".
